% Author: Alfredo SÃ¡nchez Alberca (asalber@ceu.es)
\section*{Integrals}
\small
\tcbset{enhanced, colback=color1!10, colframe=color1, fonttitle=\bfseries\large\sffamily, %lifted shadow={1mm}{-2mm}{3mm}{0.1mm}
}

\begin{multicols}{2}
\begin{tcolorbox}[hbox, title=Basic antiderivatives]
\begin{minipage}{0.4\textwidth}
\begin{description}
  \item[Powers]
  \[
    \int a\,dx=ax+C
  \]
  \[
    \int x^n\,dx=\dfrac{x^{n+1}}{n+1}+C
  \]
  \item[Exponentials]
  \[
    \int e^x\,dx=e^x+C.
  \]
  \[
    \dint a^x\,dx=\dfrac{a^x}{\ln(a)}+C
  \]
  \item[Logarithms]
  \[
    \int \dfrac{1}{x}\, dx=\ln|x|+C
  \]
  \item[Trigonometrics]
  \[
    \int \sin(x)\, dx=-\cos(x)+C
  \]
  \[
    \int \cos(x)\, dx=\sin(x)+C
  \]
  \[
    \int \frac{1}{\cos(x)^2}\, dx = \tan(x)+C
  \]
  \[
    \int \tan(x)\, dx=\ln|\sec(x)|+C
  \]
  \[
    \int \sec(x)\, dx = \ln|\sec(x) + \tan(x)|+C
  \]
  \[
    \int \csc(x)\, dx= \ln|\csc(x)-\cot(x)|+C
  \] 
  \[
    \int \cot(x) \, dx= \ln|\sin(x)|+C
  \] 
  \[
    \int \sec(x)^2\, dx= \tan(x)+ C
  \] 
  \[
    \int \csc(x)^2\, dx= -\cot(x)+ C
  \] 
  \[
    \int \sec(x)\tan(x)\, dx= \sec(x)+ C
  \] 
  \[
    \int \csc(x)\cot(x)\, dx = -\csc(x) +C
  \]
  \item[Rationals e irrationals]
  \[
    \int\frac{dx}{\sqrt{a^2-x^2}}=\sin^{-1}\left(\frac{x}{a}\right)+C
  \] 
  \[
    \int\frac{dx}{a^2+x^2}=\frac{1}{a}\tan^{-1}\left(\dfrac{x}{a}\right)+C
  \] 
  \[
    \int\dfrac{dx}{x\sqrt{x^2-a^2}}=\frac{1}{a}\sec^{-1}\left(\dfrac{x}{a}\right)+C
  \] 
  \[
    \int\frac{dx}{a^2-x^2}=\frac{1}{2a}\ln\left|\frac{x+a}{x-a}\right|+C
  \]
\end{description}
\end{minipage}
\end{tcolorbox}

\begin{tcolorbox}[hbox, title=Integration rules]
  \begin{minipage}{0.4\textwidth}
    \begin{description}
      \item[Sum]
      \[
        \int u+v\,dx = \int u\,dx + \int v\,dx
      \]
      \item[Difference]
      \[
        \int u-v\,dx = \int u\,dx - \int v\,dx
      \]
      \item[Product by a constant]
      \[
        \int af(x)\,dx = a\int f(x)\,dx
      \]
      \item[Parts]
      \[
        \int u\,dv = uv - \int v\,du
      \]
      \item[Substitution]
      \[
        \int f(u)u'\,dx = \int f(u)\,du
      \]
    \end{description}
  \end{minipage}
\end{tcolorbox}

\begin{tcolorbox}[hbox, title=Definite integrals]
  \begin{minipage}{0.4\textwidth}
    \begin{description}
      \item[Barrow's rule]
      \[
        \int_a^b f(x)\,dx = F(b)-F(a)
      \]
      where $F(x) = \int f(x)\,dx$
      \begin{center}
      \input{img/area_positive_function}
      \end{center}
      \item[Properties]
      \[
        \int_a^a f(x)\,dx = 0
      \]
      \[
        \int_a^b f(x)\,dx = -\int_b^a f(x)\,dx
      \]
      \[
        \int_a^b f(x)\, dx = \int_a^c f(x)\,dx + \int_c^b f(x)\,dx
      \]
      where $a<c<b$.
    \end{description}
  \end{minipage}
\end{tcolorbox}
\end{multicols}